Cvc/Srt/SrtBij.lean
@@ -1,0 +1,101 @@
+/-
+Copyright (c) 2023-2025 by the authors listed in the file AUTHORS and their
+institutional affiliations. All rights reserved.
+Released under Apache 2.0 license as described in the file LICENSE.
+Authors: Adrien Champion
+-/
+
+import Cvc.Srt.Defs
+import Cvc.Srt.Types
+
+
+
+/-! # Relates `Srt`-s to `Type`-s
+
+Main class `Srt.Bij (α : Type)` associates `srt : Srt` to `α`. It guarantees this association works
+both ways by asking for a proof that `α = srt.toType`.
+-/
+namespace Cvc
+
+
+
+/-- Denotes a *"bijection"* from the `α` type itself (not its values) to `Srt`.
+
+*"Bijection"* here means that when `A : SrtBij α`, then `A.srt.toType = α` as guaranteed by `valid`.
+-/
+protected class Srt.Bij (α : Type) where private mk ::
+  /-- `Srt` version of `α`. -/
+  srt : Srt
+  /-- Turning `srt` into a `Type` results in `α`. -/
+  h_bij : α = srt.toType := by
+    simp [toType, Srt.Bij.h_bij, *] <;> rfl
+
+/-- Retrieves the `Srt` corresponding to a `Type`. -/
+abbrev getSrt (α : Type) [I : Srt.Bij α] : Srt :=
+  I.srt
+
+namespace Srt
+
+@[inherit_doc getSrt]
+abbrev ofType := Cvc.getSrt
+
+namespace Bij
+
+/-! ## Instances for simple types -/
+
+instance instUnit : Srt.Bij Unit := mk .unit
+instance instBool : Srt.Bij Bool := mk .bool
+instance instInt : Srt.Bij Int := mk .int
+instance instRat : Srt.Bij Rat := mk .real
+instance instString : Srt.Bij String := mk .string
+instance instRoundingMode : Srt.Bij Cvc.RoundingMode := mk <| .roundingMode
+instance instRegex : Srt.Bij Cvc.Regex := mk <| .regex
+
+/-! ## Instances for non-`Srt`-parameterized types -/
+instance instAnyFloat : Srt.Bij (Cvc.AnyFloat exp sig) := mk <| .float exp sig
+instance instAbstract : Srt.Bij (Cvc.Abstract k) := mk <| .abstract k
+instance instFiniteField : Srt.Bij (Cvc.FiniteField n) := mk <| .finiteField n
+
+/-! ## Instances composite types -/
+section variable [A : Srt.Bij α] [B : Srt.Bij β]
+
+instance instArray : Srt.Bij (Array α) := mk <| .seq A.srt
+instance instBitVec : Srt.Bij (BitVec size) := mk <| .bitVec size
+instance instFunction : Srt.Bij (α → β) := mk <| .function A.srt B.srt
+instance instProd : Srt.Bij (α × β) := mk <| .prod A.srt B.srt
+instance instTMap : Srt.Bij (Cvc.TMap α β) := mk <| .array A.srt B.srt
+instance instBag : Srt.Bij (Cvc.Bag α) := mk <| .bag A.srt
+instance instSet : Srt.Bij (Cvc.Set α) := mk <| .set A.srt
+instance instUninterpreted : Srt.Bij (Uninterpreted α) := mk <| .uninterpreted A.srt
+
+end
+
+end Bij
+end Srt
+
+
+
+/-! ## Refinement of `Srt.Bij` to arithmetic sorts -/
+
+/-- Proof that the sort associated to `α` is arithmetic. -/
+protected abbrev is_arith (α : Type) [Srt.Bij α] :=
+  Srt.ofType α |>.is_arith
+
+namespace Srt.Bij
+
+/-- Extends `Srt.Bij` with a proof that `α`'s `Srt` is arithmetic. -/
+protected class Arith (α : Type) extends Srt.Bij α where
+  /-- Sort `srt` is an arithmetic sort. -/
+  h_arith : Cvc.is_arith α := by simp
+
+namespace Arith
+
+example [Srt.Bij.Arith α] : Srt.Bij α := inferInstance
+
+/-! ## Instances for `Int` and `Rat` (`Real`) -/
+instance instInt : Bij.Arith Int := {}
+instance instRat : Bij.Arith Rat := {}
+
+end Arith
+
+end Srt.Bij
