Tests/Terms/Basic.lean
@@ -1,0 +1,76 @@
+/-
+Copyright (c) 2023-2025 by the authors listed in the file AUTHORS and their
+institutional affiliations. All rights reserved.
+Released under Apache 2.0 license as described in the file LICENSE.
+Authors: Adrien Champion
+-/
+
+import Tests.Basic
+
+
+
+namespace Cvc.Test
+
+
+
+Term.test!
+
+with
+  let boo ← Term.bool false
+  let seven ← Term.int 7
+  let five ← Term.int 5
+  let ten ← Term.int 10
+  show[", "| boo, seven, five, ten]
+
+
+[Term.equal]
+  let equal_7_5_10 ← Term.mkEqual #[seven, five, ten]
+  let equal_5_10 ← Term.mkEqual #[five, ten]
+  let seven_equal_five ← seven.equal five
+  show[equal_7_5_10, equal_5_10, seven_equal_five]
+/-- info: boo ↦ false, seven ↦ 7, five ↦ 5, ten ↦ 10
+
+equal_7_5_10 ↦ (and (= 7 5) (= 5 10))
+equal_5_10 ↦ (= 5 10)
+seven_equal_five ↦ (= 7 5)
+-/
+
+[Term.distinct]
+  let distinct_7_5_10 ← Term.mkDistinct #[seven, five, ten]
+  let distinct_5_10 ← Term.mkDistinct #[five, ten]
+  let seven_distinct_five ← seven.distinct five
+  show[distinct_7_5_10, distinct_5_10, seven_distinct_five]
+/-- info: boo ↦ false, seven ↦ 7, five ↦ 5, ten ↦ 10
+
+distinct_7_5_10 ↦ (distinct 7 5 10)
+distinct_5_10 ↦ (distinct 5 10)
+seven_distinct_five ↦ (distinct 7 5)
+-/
+
+[Term.ite]
+  let if_boo_seven_five ← boo.ite seven five
+  show[if_boo_seven_five]
+/-- info: boo ↦ false, seven ↦ 7, five ↦ 5, ten ↦ 10
+
+if_boo_seven_five ↦ (ite false 7 5)
+-/
+
+[Term.mul]
+  let mul_7_5_10 ← Term.mkMul #[seven, five, ten]
+  let seven_mul_five ← seven.mul five
+  show[mul_7_5_10, seven_mul_five]
+/-- info: boo ↦ false, seven ↦ 7, five ↦ 5, ten ↦ 10
+
+mul_7_5_10 ↦ (* 7 5 10)
+seven_mul_five ↦ (* 7 5)
+-/
+
+[Term.add]
+  let add_7_5_10 ← Term.mkAdd #[seven, five, ten]
+  let seven_add_five ← seven.add five
+  show[add_7_5_10, seven_add_five]
+/-- info: boo ↦ false, seven ↦ 7, five ↦ 5, ten ↦ 10
+
+add_7_5_10 ↦ (+ 7 5 10)
+seven_add_five ↦ (+ 7 5)
+-/
