Tests/Terms/CompileFail.lean
@@ -1,0 +1,65 @@
+/-
+Copyright (c) 2023-2025 by the authors listed in the file AUTHORS and their
+institutional affiliations. All rights reserved.
+Released under Apache 2.0 license as described in the file LICENSE.
+Authors: Adrien Champion
+-/
+import Cvc.Defs
+import Tests.Basic
+
+
+
+namespace Cvc.Test
+
+
+
+Term.test!
+
+
+[Term.mkEqual.noArg]
+  Term.mkEqual #[]
+/-- error: could not synthesize default value for parameter 'h_size' using tactics
+---
+error: expected an array of **at least** two terms
+⊢ 2 ≤ #[].size
+-/
+
+[Term.mkDistinct.oneArg]
+  let seven ← Term.int 7
+  -- all of type `Term Bool`
+  Term.mkEqual #[seven]
+/--
+error: could not synthesize default value for parameter 'h_size' using tactics
+---
+error: expected an array of **at least** two terms
+seven : Term.Int
+⊢ 2 ≤ #[seven].size
+-/
+
+[Term.mkAdd.nonArith]
+  let b1 ← Term.bool true
+  let b2 ← Term.bool false
+  let b3 ← Term.bool false
+  let b4 ← Term.bool false
+  -- all of type `Term Bool`
+  Term.mkAdd #[b1, b2, b3, b4]
+/--
+error: could not synthesize default value for parameter 'h_arith' using tactics
+---
+error: expected arithmetic type `Int` or `Rat`, see `Cvc.is_arith` and `Cvc.Srt.Bij.Arith`
+b1 b2 b3 b4 : Term.Bool
+⊢ Cvc.is_arith Bool
+-/
+
+[Term.add.nonArith]
+  let b1 ← Term.bool true
+  let b2 ← Term.bool false
+  -- all of type `Term Bool`
+  b1.add b2
+/--
+error: could not synthesize default value for parameter 'h_arith' using tactics
+---
+error: expected arithmetic type `Int` or `Rat`, see `Cvc.is_arith` and `Cvc.Srt.Bij.Arith`
+b1 b2 : Term.Bool
+⊢ Cvc.is_arith Bool
+-/
